<?xml version="1.0" encoding="utf-8"?>
<rdf:RDF
   xmlns:bibo="http://purl.org/ontology/bibo/"
   xmlns:co="http://purl.org/ontology/co/core#"
   xmlns:dc="http://purl.org/dc/elements/1.1/"
   xmlns:frbr="http://purl.org/vocab/frbr/core#"
   xmlns:olo="http://purl.org/ontology/olo/core#"
   xmlns:owl="http://www.w3.org/2002/07/owl#"
   xmlns:pbo="http://purl.org/ontology/pbo/core#"
   xmlns:rdf="http://www.w3.org/1999/02/22-rdf-syntax-ns#"
   xmlns:rdfs="http://www.w3.org/2000/01/rdf-schema#"
   xmlns:vs="http://www.w3.org/2003/06/sw-vocab-status/ns#"
   xmlns:xsd="http://www.w3.org/2001/XMLSchema#">
  <owl:Ontology rdf:about="http://purl.org/ontology/pbo/core#">
    <dc:creator rdf:resource="http://foaf.me/zazi#me"/>
    <dc:date rdf:datatype="http://www.w3.org/2001/XMLSchema#dateTime">2010-07-19T20:10:52+01:00</dc:date>
    <dc:description xml:lang="en">The Play Back Ontology specification provides basic concepts and properties 
for describing a concepts that are related to the play back domain, e.g. an playlist, play back count and skip counter 
on/ for the Semantic Web. This document contains a RDF description of the Play Back Ontology.</dc:description>
    <dc:title xml:lang="en">The Play Back Ontology</dc:title>
    <owl:imports rdf:resource="http://purl.org/dc/elements/1.1/"/>
    <owl:imports rdf:resource="http://purl.org/ontology/bibo/"/>
    <owl:imports rdf:resource="http://purl.org/ontology/co/core"/>
    <owl:imports rdf:resource="http://purl.org/ontology/olo/core"/>
    <owl:imports rdf:resource="http://www.w3.org/2003/06/sw-vocab-status/ns"/>
    <owl:versionInfo rdf:datatype="http://www.w3.org/2001/XMLSchema#decimal">0.1</owl:versionInfo>
  </owl:Ontology>
  <owl:Class rdf:about="http://purl.org/ontology/pbo/core#PlayBackCounter">
    <rdfs:comment xml:lang="en">A play back counter of a specific object. A play back counter is related to  specific co:ScrobbleEvent instances, which 
are the related play back events of an object.</rdfs:comment>
    <rdfs:isDefinedBy rdf:resource="http://purl.org/ontology/pbo/core#"/>
    <rdfs:label xml:lang="en">Play Back Counter</rdfs:label>
    <rdfs:subClassOf rdf:resource="http://purl.org/ontology/co/core#Counter"/>
    <vs:term_status xml:lang="en">unstable</vs:term_status>
  </owl:Class>
  <owl:Class rdf:about="http://purl.org/ontology/pbo/core#Playlist">
    <rdfs:comment xml:lang="en">A playlist of specific media items, e.g. music tracks, videos or slides.</rdfs:comment>
    <rdfs:isDefinedBy rdf:resource="http://purl.org/ontology/pbo/core#"/>
    <rdfs:label xml:lang="en">Playlist</rdfs:label>
    <rdfs:subClassOf rdf:resource="http://purl.org/ontology/olo/core#OrderedList"/>
    <vs:term_status xml:lang="en">unstable</vs:term_status>
  </owl:Class>
  <owl:Class rdf:about="http://purl.org/ontology/pbo/core#PlaylistSlot">
    <rdfs:comment xml:lang="en">A playlist slot. It could contain e.g. a music track, a video or a slide, and maybe related with some 
additional properties. However, it could maybe also included a "sub" playlist, e.g. to keep a fixed sequence of some tracks.</rdfs:comment>
    <rdfs:isDefinedBy rdf:resource="http://purl.org/ontology/pbo/core#"/>
    <rdfs:label xml:lang="en">Playlist Slot</rdfs:label>
    <rdfs:subClassOf rdf:resource="http://purl.org/ontology/olo/core#Slot"/>
    <vs:term_status xml:lang="en">testing</vs:term_status>
  </owl:Class>
  <owl:Class rdf:about="http://purl.org/ontology/pbo/core#SkipCounter">
    <rdfs:comment xml:lang="en">A skip counter of a specific object. A skip counter is related to  specific co:ScrobbleEvent instances, which 
are the related skip events of an object.</rdfs:comment>
    <rdfs:isDefinedBy rdf:resource="http://purl.org/ontology/pbo/core#"/>
    <rdfs:label xml:lang="en">Skip Counter</rdfs:label>
    <rdfs:subClassOf rdf:resource="http://purl.org/ontology/co/core#Counter"/>
    <vs:term_status xml:lang="en">unstable</vs:term_status>
  </owl:Class>
  <rdf:Property rdf:about="http://purl.org/ontology/pbo/core#occasion">
    <rdfs:comment xml:lang="en">An occasion for which a playlist was created.</rdfs:comment>
    <rdfs:domain rdf:resource="http://purl.org/ontology/pbo/core#Playlist"/>
    <rdfs:isDefinedBy rdf:resource="http://purl.org/ontology/pbo/core#"/>
    <rdfs:label xml:lang="en">has occassion</rdfs:label>
    <owl:inverseOf>
      <rdf:Property>
        <rdfs:label xml:lang="en">is occassion of</rdfs:label>
      </rdf:Property>
    </owl:inverseOf>
    <vs:term_status xml:lang="en">unstable</vs:term_status>
  </rdf:Property>
  <owl:ObjectProperty rdf:about="http://purl.org/ontology/pbo/core#playlist_item">
    <rdfs:comment xml:lang="en">A specific playlist item, e.g. a music track, video or slides. The range types of this property must be 
based on bibo:Document or frbr:Endeavour (to keep it somehow media based).</rdfs:comment>
    <rdfs:domain rdf:resource="http://purl.org/ontology/pbo/core#PlaylistSlot"/>
    <rdfs:isDefinedBy rdf:resource="http://purl.org/ontology/pbo/core#"/>
    <rdfs:label xml:lang="en">has playlist item</rdfs:label>
    <rdfs:range>
      <rdf:Description>
        <owl:unionOf>
          <rdf:Description>
            <rdf:first rdf:resource="http://purl.org/ontology/bibo/Document"/>
            <rdf:rest>
              <rdf:Description>
                <rdf:first rdf:resource="http://purl.org/vocab/frbr/core#Endeavour"/>
                <rdf:rest>
                  <rdf:Description>
                    <rdf:first rdf:resource="http://purl.org/ontology/pbo/core#PlaylistSlot"/>
                    <rdf:rest rdf:resource="http://www.w3.org/1999/02/22-rdf-syntax-ns#nil"/>
                  </rdf:Description>
                </rdf:rest>
              </rdf:Description>
            </rdf:rest>
          </rdf:Description>
        </owl:unionOf>
      </rdf:Description>
    </rdfs:range>
    <rdfs:subPropertyOf rdf:resource="http://purl.org/ontology/olo/core#item"/>
    <owl:inverseOf>
      <owl:ObjectProperty>
        <rdfs:label xml:lang="en">is playlist item of</rdfs:label>
      </owl:ObjectProperty>
    </owl:inverseOf>
    <vs:term_status xml:lang="en">unstable</vs:term_status>
  </owl:ObjectProperty>
</rdf:RDF>
